Verifying interpreter incrementally. Store verified

examples/sgx/verify/VerSGXState.fst
@@ -2,7 +2,7 @@
 module VerSGXState
 
 open FStar.UInt64
-open Ast
+open VerAst
 
 
 type cpuregstate =
@@ -40,3 +40,23 @@ let search_reg (regname:string) (env:cpuregstate) :(Tot dword) =
 let read (regname:string) (env:cpuregstate) :(Tot dword)  =
 	search_reg regname (env)
 
+val update: string -> dword->cpuregstate->Tot cpuregstate
+let update (regname:string) (value:dword) (env:cpuregstate) =
+	if regname = "rsp" then
+		{env with rsp=value}
+	else if regname = "rbp" then
+		{env with rbp=value}
+	else if regname = "rax" then
+		{env with rax=value}
+	else if regname = "rbx" then
+		{env with rbx=value}
+	else if regname = "rcx" then
+		{env with rcx=value}
+	else if regname = "rdx" then
+		{env with rdx=value}
+	else if regname = "r8" then
+		{env with r8=value}
+	else 
+		{env with r9=value}
+	
+						
